proof/Russell/Axioms.v
@@ -4,6 +4,12 @@ Require Import Conv.
 Require Import LiftSubst.
 Require Import Env.
 Require Import CCPD.Types.
+Require Import CCPD.Thinning.
+Require Import CCPD.Substitution.
+Require Import CCPD.Coercion.
+Require Import CCPD.GenerationNotKind.
+Require Import CCPD.GenerationCoerce.
+Require Import CCPD.Generation.
 
 Implicit Types i k m n p : nat.
 Implicit Type s : sort.
@@ -12,19 +18,86 @@ Implicit Types e f g : env.
 
 Set Implicit Arguments.
 
-Axiom inv_conv_prod_sort_l : forall e U V U' V' s, e |- Prod U V : Srt s -> e |- Prod U' V' : Srt s ->
-  conv (Prod U V) (Prod U' V') -> { s1 : sort | e |- U : Srt s1 /\ e |- U' : Srt s1 }. 
+Axiom unique_sort_conv : forall G A A' s1 s2, G |- A : Srt s1 -> G |- A' : Srt s2 -> conv A A' -> s1 = s2.
 
-Axiom inv_conv_prod_sort_r : forall e U V U' V' s, e |- Prod U V : Srt s -> e |- Prod U' V' : Srt s ->
+Lemma inv_conv_prod_sort_l : forall e U V U' V' s, e |- Prod U V : Srt s -> e |- Prod U' V' : Srt s ->
+  conv (Prod U V) (Prod U' V') -> exists s1 : sort, e |- U : Srt s1 /\ e |- U' : Srt s1 .
+Proof.
+  intros.
+  destruct (generation_prod2 H).
+  destruct (generation_prod2 H0).
+  destruct H2 ; destruct H4.
+  pose (inv_conv_prod_l _ _ _ _ H1).
+  pose (inv_conv_prod_r _ _ _ _ H1).
+  pose (unique_sort_conv H2 H4 c).
+  exists x.
+  split ; intuition.
+  rewrite e0 ; assumption.
+Qed.
+
+Lemma inv_conv_prod_sort_r : forall e U V U' V' s, e |- Prod U V : Srt s -> e |- Prod U' V' : Srt s ->
   conv (Prod U V) (Prod U' V') -> U' :: e |- V : Srt s /\ U' :: e |- V' : Srt s. 
+Proof.
+  intros.
+  destruct (generation_prod2 H).
+  destruct (generation_prod2 H0).
+  destruct H2 ; destruct H4.
+  pose (inv_conv_prod_l _ _ _ _ H1).
+  pose (inv_conv_prod_r _ _ _ _ H1).
+  pose (unique_sort_conv H2 H4 c).
+  intuition.
+  apply typ_conv_env with (U :: e) ; auto with coc.
+  apply coerce_env_hd with x0.
+  apply coerce_conv with U' U'; auto with coc.
+  rewrite <- e0 ; auto.
+  apply wf_var with x0 ; auto.
+Qed.
 
-Axiom inv_conv_sum_sort_l : forall e U V U' V' s, e |- Sum U V : Srt s -> e |- Sum U' V' : Srt s ->
-  conv (Sum U V) (Sum U' V') -> { s1 : sort | e |- U : Srt s1 /\ e |- U' : Srt s1 }. 
-
-Axiom inv_conv_sum_sort_r : forall e U V U' V' s, e |- Sum U V : Srt s -> e |- Sum U' V' : Srt s ->
-  conv (Sum U V) (Sum U' V') -> U :: e |- V : Srt s /\ U :: e |- V' : Srt s.
-
-Axiom inv_conv_sum_sort : forall e U V U' V' s, e |- Sum U V : Srt s -> e |- Sum U' V' : Srt s ->
+Lemma inv_conv_sum_sort : forall e U V U' V' s, e |- Sum U V : Srt s -> e |- Sum U' V' : Srt s ->
   conv (Sum U V) (Sum U' V') -> 
   exists s1, exists s2, e |- U : Srt s1 /\ e |- U' : Srt s1 /\ U :: e |- V : Srt s2 /\ U :: e |- V' : Srt s2
-  /\ sum_sort s1 s2 s.	        
+  /\ sum_sort s1 s2 s.	
+Proof. 
+  intros.
+  destruct (generation_sum2 H).
+  destruct (generation_sum2 H0).
+  destruct H2 ; destruct H3.
+  destruct H4 ; destruct H5.
+  intuition.
+  pose (inv_conv_sum_l _ _ _ _ H1).
+  pose (inv_conv_sum_r _ _ _ _ H1).
+  pose (unique_sort_conv H2 H3 c).
+  rewrite <- e0 in H3.
+  exists x ; exists x1 ; intuition.
+
+
+  cut (U :: e |- V' : Srt x2) ; intros.
+  pose (unique_sort_conv H6 H9 c0).
+  rewrite e1 ; auto.
+
+  apply typ_conv_env with (U' :: e) ; auto with coc.
+  apply coerce_env_hd with x ; auto with coc.
+  apply coerce_conv with U U ; auto with coc.
+  apply wf_var with x ; auto with coc.
+Qed.
+
+(* Set versions of the lemmas derived from the axiom *)
+Axiom inv_conv_prod_sort_l_set : forall e U V U' V' s, e |- Prod U V : Srt s -> e |- Prod U' V' : Srt s ->
+  conv (Prod U V) (Prod U' V') -> { s1 : sort | e |- U : Srt s1 /\ e |- U' : Srt s1 }.
+
+
+Axiom inv_conv_prod_sort_r_set : forall e U V U' V' s, e |- Prod U V : Srt s -> e |- Prod U' V' : Srt s ->
+  conv (Prod U V) (Prod U' V') -> U' :: e |- V : Srt s /\ U' :: e |- V' : Srt s. 
+
+Axiom inv_conv_sum_sort_set : forall e U V U' V' s, e |- Sum U V : Srt s -> e |- Sum U' V' : Srt s ->
+  conv (Sum U V) (Sum U' V') -> 
+  { s1 : sort & { s2 : sort | e |- U : Srt s1 /\ e |- U' : Srt s1 /\ U :: e |- V : Srt s2 /\ U :: e |- V' : Srt s2
+  /\ sum_sort s1 s2 s}}.	
+
+Axiom inv_conv_sum_sort_l_set : forall e U V U' V' s, e |- Sum U V : Srt s -> e |- Sum U' V' : Srt s ->
+  conv (Sum U V) (Sum U' V') -> 
+  { s1 : sort | e |- U : Srt s1 /\ e |- U' : Srt s1 }.
+
+Axiom inv_conv_sum_sort_r_set : forall e U V U' V' s, e |- Sum U V : Srt s -> e |- Sum U' V' : Srt s ->
+  conv (Sum U V) (Sum U' V') -> 
+  { s2 : sort | U :: e |- V : Srt s2 /\ U :: e |- V' : Srt s2 }.
